Cleaner and nicer example, demonstrating more things :)

ind/Example.fst
@@ -4,14 +4,19 @@ module HS = FStar.HyperStack
 module HST = FStar.HyperStack.ST
 module B = LowStar.Buffer
 module DLL = DoublyLinkedListIface
+module L = FStar.List.Tot
 
-let main () : HST.Stack unit (fun _ -> True) (fun _ _ _ -> True) =
+let main () : HST.Stack (unit) (fun _ -> True) (fun _ _ _ -> True) =
   let open DLL in
   HST.push_frame ();
   let d : dll UInt32.t = dll_new () in
   let n1 = node_of 1ul in
-  // let h0 = HST.get () in assert (g_node_val h0 n1 = 1ul);
   let n2 = node_of 2ul in
-  // let h1 = HST.get () in assert (g_node_val h1 n1 = 1ul); assert (g_node_val h1 n2 = 2ul);
   dll_insert_at_head d n1;
+  dll_insert_at_tail d n2;
+  let h0 = HST.get () in
+  let n1' = dll_head d in
+  let t = node_val n1' in
+  assert (node_valid h0 n1);
+  assert (t == 1ul);
   HST.pop_frame ()
